Prove substP_distr_addPP. Begin working on substP_distr_mulPP, the last remaining admitted lemma!

B_Unification/poly_unif.v
@@ -4,6 +4,7 @@ Import ListNotations.
 Require Import Arith.
 Require Import Permutation.
 Require Import Sorting.
+Import Nat.
 
 Require Export poly.
 
@@ -32,19 +33,16 @@ Fixpoint substM (s : subst) (m : mono) : poly :=
 Lemma substM_is_poly : forall s m,
   is_poly (substM s m).
 Proof.
-  intros s m. destruct m; simpl; auto.
+  intros s m. unfold substM; destruct m; auto.
 Qed.
 
-Fixpoint substP (s : subst) (p : poly) : poly :=
-  match p with
-  | [] => []
-  | m :: p' => addPP (substM s m) (substP s p')
-  end.
+Definition substP (s : subst) (p : poly) : poly :=
+  make_poly (concat (map (substM s) p)).
 
 Lemma substP_is_poly : forall s p,
   is_poly (substP s p).
 Proof.
-  intros. unfold substP. destruct p; auto.
+  intros. unfold substP. auto.
 Qed.
 
 Hint Resolve substP_is_poly substM_is_poly.
@@ -52,156 +50,20 @@ Hint Resolve substP_is_poly substM_is_poly.
 Lemma substP_Sorted : forall s p,
   Sorted (fun m n : list nat => lex Nat.compare m n = Lt) (substP s p).
 Proof.
-  intros s p. destruct p.
-  - simpl. auto.
-  - simpl. apply addPP_is_poly.
+  intros s p. apply substP_is_poly.
 Qed.
 
 Lemma make_poly_Permutation : forall p q,
   Permutation p q ->
   Permutation (make_poly p) (make_poly q).
 Proof.
-  intros p q H. unfold make_poly. apply Permutation_trans with (l':=(nodup_cancel mono_eq_dec (map make_mono p))).
+  intros p q H. unfold make_poly. apply Permutation_trans with (l':=(nodup_cancel 
+    mono_eq_dec (map make_mono p))).
   - apply Permutation_sym. apply MonoSort.Permuted_sort.
   - apply Permutation_trans with (l':=(nodup_cancel mono_eq_dec (map make_mono q))).
     + apply nodup_cancel_Permutation. apply Permutation_map. apply H.
     + apply MonoSort.Permuted_sort.
 Qed.
-
-Lemma substP_Permutation : forall s p q,
-  Permutation p q ->
-  Permutation (substP s p) (substP s q).
-Proof.
-  intros s p q H. induction H.
-  - simpl. auto.
-  - simpl. unfold addPP. apply make_poly_Permutation.
-    apply Permutation_app_head. apply IHPermutation.
-  - simpl. rewrite <- addPP_assoc; auto. rewrite <- addPP_assoc; auto.
-    rewrite (addPP_comm (substM _ _)). apply Permutation_refl.
-  - apply Permutation_trans with (l':=(substP s l')); auto.
-Qed.
-
-Lemma substP_sort_assoc : forall s p,
-  substP s (MonoSort.sort p) = MonoSort.sort (substP s p).
-Proof.
-  intros s p. apply Permutation_Sorted_eq.
-  - apply Permutation_trans with (l':=(substP s p)).
-    + apply substP_Permutation. apply Permutation_sym. apply MonoSort.Permuted_sort.
-    + apply MonoSort.Permuted_sort.
-  - apply Sorted_MonoSorted. apply substP_Sorted.
-  - apply MonoSort.LocallySorted_sort.
-Qed.
-
-Lemma count_occ_substP : forall s a p,
-  forall m, In m (substM s a) ->
-  count_occ mono_eq_dec (substP s (a::p)) m =
-  (count_occ mono_eq_dec (a::p) a + count_occ mono_eq_dec (a::p) m)%nat.
-Proof.
-Admitted.
-
-Definition list_parity_match (p q:poly) m : Prop :=
-  Nat.even (count_occ mono_eq_dec p m) = Nat.even (count_occ mono_eq_dec q m).
-
-Lemma incl_parity_Permutation : forall l m,
-  incl l m -> 
-  incl m l ->
-  (forall x, In x l -> list_parity_match l m x) ->
-  Permutation (nodup_cancel mono_eq_dec l) (nodup_cancel mono_eq_dec m).
-Proof.
-Admitted.
-
-Lemma incl_remove_nodup_cancel : forall s p a,
-  incl (substP s (remove mono_eq_dec a (nodup_cancel mono_eq_dec p))) (substP s p).
-Proof.
-  intros s p a m Hin. induction p.
-  - simpl. auto.
-  - simpl in *.
-Admitted.
-
-Lemma substP_nodup_cancel_assoc : forall s p,
-  substP s (nodup_cancel mono_eq_dec p) = 
-  nodup_cancel mono_eq_dec (substP s p).
-Proof.
-  intros s p. apply Permutation_Sorted_eq.
-  - rewrite (no_nodup_cancel_NoDup _ _ (substP _ _)).
-    + induction p.
-      * auto.
-      * simpl. destruct Nat.even eqn:Hevn.
-        -- simpl. unfold addPP. unfold make_poly. rewrite <- Permutation_MonoSort_l.
-           rewrite <- Permutation_MonoSort_r. repeat rewrite no_map_make_mono.
-           apply incl_parity_Permutation.
-           ++ apply incl_app. intuition. apply incl_appr. unfold incl.
-              apply incl_remove_nodup_cancel.
-           ++ admit.
-           ++ admit.
-           ++ intros m Hin. apply in_app_iff in Hin. destruct Hin.
-              apply (substM_is_poly s a); auto.
-              apply (substP_is_poly s p); auto.
-           ++ intros m Hin. apply in_app_iff in Hin. destruct Hin.
-              apply (substM_is_poly s a); auto.
-              apply (substP_is_poly s (remove mono_eq_dec a (nodup_cancel mono_eq_dec p))); auto.
-        -- admit. (* destruct remove eqn:Hrem.
-           ++ admit.
-           ++ simpl. unfold addPP, make_poly. apply Permutation_MonoSort_r.
-              apply Permutation_MonoSort_l. repeat rewrite no_map_make_mono.
-              apply incl_parity_Permutation.
-              ** admit.
-              ** admit.
-              ** intros x Hin. admit.
-              ** intros m Hin. apply in_app_iff in Hin. destruct Hin.
-                 apply (substM_is_poly s a); auto.
-                 apply (substP_is_poly s p); auto.
-              ** intros m Hin. apply in_app_iff in Hin. destruct Hin.
-                 apply (substM_is_poly s l); auto.
-                 apply (substP_is_poly s l0); auto. *)
-    + pose (substP_is_poly s p). unfold is_poly in i. destruct i. apply NoDup_MonoSorted. auto.
-  - apply Sorted_MonoSorted. apply substP_Sorted.
-  - apply Sorted_nodup_cancel. apply MonoOrder_Transitive.
-    apply Sorted_MonoSorted. apply substP_Sorted.
-Admitted.
-
-Lemma substP_make_poly_assoc : forall s p,
-  (forall m, In m p -> is_mono m) ->
-  substP s (make_poly p) = make_poly (substP s p).
-Proof.
-  intros s p Hmono. destruct p as [|a].
-  - simpl. auto.
-  - simpl. rewrite (no_make_poly (addPP _ _)); auto. unfold addPP, make_poly in *.
-    repeat rewrite no_map_make_mono; auto. rewrite substP_sort_assoc.
-    apply Permutation_sort_eq. rewrite substP_nodup_cancel_assoc. simpl.
-    unfold addPP, make_poly. rewrite sort_nodup_cancel_assoc.
-    rewrite no_nodup_cancel_NoDup. rewrite no_map_make_mono.
-    + apply nodup_cancel_Permutation. apply Permutation_sym. apply MonoSort.Permuted_sort.
-    + intros m Hin. apply in_app_or in Hin. destruct Hin.
-      * pose (substM_is_poly s a). unfold is_poly in i. destruct i. auto.
-      * pose (substP_is_poly s p). unfold is_poly in i. destruct i. auto.
-    + apply NoDup_nodup_cancel.
-    + intros m Hin. apply in_app_or in Hin. destruct Hin.
-      * pose (substM_is_poly s a). unfold is_poly in i. destruct i. auto.
-      * pose (substP_is_poly s p). unfold is_poly in i. destruct i. auto.
-Qed.
-
-Lemma substP_distr_app : forall p q s,
-  substP s (p ++ q) = addPP (substP s p) (substP s q).
-Proof.
-  intros p q s. induction p.
-  - simpl. rewrite addPP_0; auto.
-  - simpl. rewrite addPP_assoc; auto. rewrite IHp. auto.
-Qed.
-
-Lemma substP_distr_addPP : forall p q s,
-  is_poly p -> is_poly q ->
-  substP s (addPP p q) = addPP (substP s p) (substP s q).
-Proof.
-  intros p q s Hp Hq. unfold addPP. rewrite substP_make_poly_assoc.
-  - rewrite substP_distr_app. apply no_make_poly. apply make_poly_is_poly.
-  - intros m Hin. apply in_app_or in Hin as []; [apply Hp | apply Hq]; auto.
-Qed.
-
-Lemma substP_distr_mulPP : forall p q s,
-  substP s (mulPP p q) = mulPP (substP s p) (substP s q).
-Proof.
-Admitted.
 
 Lemma substM_cons : forall x m,
   ~ In x m ->
@@ -223,7 +85,8 @@ Lemma substP_cons : forall x p,
 Proof.
   intros. induction p.
   - auto.
-  - simpl. f_equal.
+  - unfold substP. simpl. repeat rewrite <- (make_poly_pointless_r _ (concat _)).
+    f_equal. f_equal.
     + apply substM_cons. apply H. left. auto.
     + apply IHp. intros. apply H. right. auto.
 Qed.
@@ -231,9 +94,237 @@ Qed.
 Lemma substP_1 : forall s,
   substP s [[]] = [[]].
 Proof.
-  intros. simpl. rewrite addPP_0r; auto.
+  intros. unfold substP. simpl. auto.
 Qed.
 
+Lemma substP_0 : forall s,
+  substP s [] = [].
+Proof.
+  intros. unfold substP. simpl. auto.
+Qed.
+
+Lemma substP_Permutation : forall s p q,
+  Permutation p q ->
+  Permutation (substP s p) (substP s q).
+Proof.
+  intros s p q H. induction H.
+  - simpl. auto.
+  - unfold substP. simpl. repeat rewrite <- (make_poly_pointless_r _ (concat _)).
+    apply make_poly_Permutation. apply Permutation_app_head. apply IHPermutation.
+  - unfold substP. simpl. apply make_poly_Permutation. repeat rewrite app_assoc.
+    apply Permutation_app_tail. apply Permutation_app_comm.
+  - apply Permutation_trans with (l':=(substP s l')); auto.
+Qed.
+
+Lemma substP_sort_assoc : forall s p,
+  substP s (MonoSort.sort p) = MonoSort.sort (substP s p).
+Proof.
+  intros s p. apply Permutation_Sorted_eq.
+  - apply Permutation_trans with (l':=(substP s p)).
+    + apply substP_Permutation. apply Permutation_sym. apply MonoSort.Permuted_sort.
+    + apply MonoSort.Permuted_sort.
+  - apply Sorted_MonoSorted. apply substP_Sorted.
+  - apply MonoSort.LocallySorted_sort.
+Qed.
+
+(* Lemma substP_make_poly_assoc : forall s p,
+  (forall m, In m p -> is_mono m) ->
+  substP s (make_poly p) = make_poly (substP s p).
+Proof.
+  intros s p Hmono. unfold substP. destruct p as [|a].
+  - simpl. auto.
+  - simpl. rewrite (no_make_poly (make_poly _)); auto. rewrite <- (app_nil_l (concat _)).
+    rewrite <- make_poly_pointless_r. simpl. unfold make_poly at 2.
+    repeat rewrite no_map_make_mono; auto. rewrite substP_sort_assoc.
+    apply Permutation_sort_eq. rewrite substP_nodup_cancel_assoc. simpl.
+    unfold addPP, make_poly. rewrite sort_nodup_cancel_assoc.
+    rewrite no_nodup_cancel_NoDup. rewrite no_map_make_mono.
+    + apply nodup_cancel_Permutation. apply Permutation_sym. apply MonoSort.Permuted_sort.
+    + intros m Hin. apply in_app_or in Hin. destruct Hin.
+      * pose (substM_is_poly s a). unfold is_poly in i. destruct i. auto.
+      * pose (substP_is_poly s p). unfold is_poly in i. destruct i. auto.
+    + apply NoDup_nodup_cancel.
+    + intros m Hin. apply in_app_or in Hin. destruct Hin.
+      * pose (substM_is_poly s a). unfold is_poly in i. destruct i. auto.
+      * pose (substP_is_poly s p). unfold is_poly in i. destruct i. auto.
+Qed.
+
+Lemma substP_distr_app : forall p q s,
+  substP s (p ++ q) = addPP (substP s p) (substP s q).
+Proof.
+  intros p q s. induction p.
+  - simpl. rewrite addPP_0; auto.
+  - unfold substP. simpl. rewrite <- make_poly_pointless_r. rewrite IHp. auto.
+Qed. *)
+
+Lemma n_le_1 : forall n,
+  n <= 1 -> n = 0 \/ n = 1.
+Proof.
+  intros n H. induction n; firstorder.
+Qed.
+
+Lemma count_occ_map_sub_not_in : forall f a p,
+  forall x, count_occ mono_eq_dec (f a) x = 0 ->
+  count_occ mono_eq_dec (concat (map f (remove mono_eq_dec a p))) x =
+  count_occ mono_eq_dec (concat (map f p)) x.
+Proof.
+  intros f a p x H. induction p as [|b]; auto. simpl.
+  rewrite count_occ_app. destruct mono_eq_dec.
+  - rewrite e in H. firstorder.
+  - simpl. rewrite count_occ_app. auto.
+Qed.
+
+Lemma count_occ_concat_map_lt : forall p a f x,
+  count_occ mono_eq_dec (f a) x  = 1 ->
+  count_occ mono_eq_dec p a <= count_occ mono_eq_dec (concat (map f p)) x.
+Proof.
+  intros p a f x H. induction p. auto. simpl. destruct mono_eq_dec.
+  - rewrite e. rewrite count_occ_app. rewrite H. simpl. firstorder.
+  - rewrite count_occ_app. induction (count_occ mono_eq_dec (f a0) x); firstorder.
+Qed.
+
+Lemma count_occ_map_sub_in : forall f a p,
+  forall x, count_occ mono_eq_dec (f a) x = 1 ->
+  count_occ mono_eq_dec (concat (map f (remove mono_eq_dec a p))) x =
+  count_occ mono_eq_dec (concat (map f p)) x - count_occ mono_eq_dec p a.
+Proof.
+  intros f a p x H. induction p as [|b]; auto. simpl. destruct mono_eq_dec.
+  - rewrite e. destruct mono_eq_dec; try contradiction. rewrite count_occ_app.
+    rewrite e in H. rewrite H. simpl. rewrite <- e. auto.
+  - simpl. destruct mono_eq_dec. symmetry in e. contradiction.
+    repeat rewrite count_occ_app. rewrite IHp. rewrite add_sub_assoc. auto.
+    apply count_occ_concat_map_lt; auto.
+Qed.
+
+Lemma f_equal_concat_sum_lt : forall f a b p x,
+  b <> a ->
+  (forall x, NoDup (f x)) ->
+  count_occ mono_eq_dec (f a) x = 1 ->
+  count_occ mono_eq_dec (f b) x = 1 ->
+  count_occ mono_eq_dec p b +
+  count_occ mono_eq_dec p a <=
+  count_occ mono_eq_dec (concat (map f p)) x.
+Proof.
+  intros f a b p x Hne Hnd Hfa Hfb. induction p as [|c]; auto. simpl.
+  destruct mono_eq_dec.
+  - rewrite e. destruct mono_eq_dec; try contradiction. rewrite count_occ_app.
+    firstorder.
+  - destruct mono_eq_dec.
+    + rewrite e. rewrite count_occ_app. firstorder.
+    + rewrite count_occ_app. pose (Hnd c). rewrite (NoDup_count_occ mono_eq_dec) in n1.
+      pose (n1 x). apply n_le_1 in l. clear n1. destruct l; firstorder.
+Qed.
+
+Lemma count_occ_nodup_concat_map_lt : forall p f a x,
+  (forall x, NoDup (f x)) ->
+  count_occ mono_eq_dec (f a) x = 1 ->
+  count_occ mono_eq_dec (nodup_cancel mono_eq_dec p) a <=
+  count_occ mono_eq_dec (concat (map f (nodup_cancel mono_eq_dec p))) x.
+Proof.
+  intros p f a x Hn H. induction p as [|b]; auto. simpl. destruct even eqn:Hev.
+  - simpl. destruct mono_eq_dec.
+    + rewrite e. rewrite count_occ_remove, count_occ_app. rewrite H. firstorder.
+    + rewrite count_occ_neq_remove; auto. rewrite not_In_remove.
+      rewrite count_occ_app. firstorder. apply not_in_nodup_cancel. auto.
+  - destruct (mono_eq_dec b a) eqn:Hba.
+    + rewrite e. rewrite count_occ_remove. firstorder.
+    + rewrite count_occ_neq_remove; auto. assert (Hn1:=(Hn b)). 
+      rewrite (NoDup_count_occ mono_eq_dec) in Hn1. assert (Hn2:=(Hn1 x)).
+      clear Hn1. apply n_le_1 in Hn2. destruct Hn2.
+      * rewrite count_occ_map_sub_not_in; auto.
+      * apply (count_occ_map_sub_in _ _ (nodup_cancel mono_eq_dec p)) in H0 as H1.
+        rewrite H1. apply le_add_le_sub_l. apply f_equal_concat_sum_lt; auto.
+Qed.
+
+Lemma nodup_cancel_concat_map : forall p f,
+  (forall x, NoDup (f x)) ->
+  Permutation
+    (nodup_cancel mono_eq_dec (concat (map f (nodup_cancel mono_eq_dec p))))
+    (nodup_cancel mono_eq_dec (concat (map f p))).
+Proof.
+  intros p f H. apply parity_nodup_cancel_Permutation. unfold parity_match.
+  intros x. induction p; auto. simpl. destruct (even (count_occ _ p a)) eqn:Hev.
+  - simpl. repeat rewrite count_occ_app. repeat rewrite even_add. rewrite not_In_remove.
+    rewrite IHp. auto. apply not_in_nodup_cancel. auto.
+  - assert (H0:=(H a)). rewrite (NoDup_count_occ mono_eq_dec) in H0.
+    assert (H1:=(H0 x)). clear H0. apply n_le_1 in H1. rewrite count_occ_app.
+    rewrite even_add. destruct H1.
+    + apply (count_occ_map_sub_not_in _ _ (nodup_cancel mono_eq_dec p)) in H0 as H1.
+      rewrite H0, H1, IHp. simpl.
+      destruct (even (count_occ _ (concat (map f p)) x)); auto.
+    + apply (count_occ_map_sub_in _ _ (nodup_cancel mono_eq_dec p)) in H0 as H1.
+      rewrite H0, H1, even_sub, IHp. simpl. rewrite count_occ_nodup_cancel. rewrite Hev.
+      destruct (even (count_occ _ (concat (map f p)) x)); auto.
+      apply count_occ_nodup_concat_map_lt; auto.
+Qed.
+
+Lemma substP_refold : forall s p,
+  make_poly (concat (map (substM s) p)) =
+  substP s p.
+Proof. auto. Qed.
+
+Lemma substP_distr_addPP : forall p q s,
+  is_poly p -> is_poly q ->
+  substP s (addPP p q) = addPP (substP s p) (substP s q).
+Proof.
+  intros p q s Hp Hq. unfold substP, addPP.
+  apply Permutation_sort_eq. apply Permutation_trans with (l':=
+    (nodup_cancel mono_eq_dec (map make_mono (concat (map (substM s) 
+    (nodup_cancel mono_eq_dec (map make_mono (p ++ q)))))))).
+    apply nodup_cancel_Permutation. apply Permutation_map. apply Permutation_concat.
+    apply Permutation_map. unfold make_poly. rewrite <- Permutation_MonoSort_l. auto.
+  apply Permutation_sym. apply Permutation_trans with (l':=(nodup_cancel 
+    mono_eq_dec (map make_mono (nodup_cancel mono_eq_dec (map make_mono (concat 
+    (map (substM s) (p)))) ++ (nodup_cancel mono_eq_dec (map make_mono (concat 
+    (map (substM s) q)))))))). apply nodup_cancel_Permutation. apply Permutation_map.
+    apply Permutation_app; unfold make_poly; rewrite <- Permutation_MonoSort_l; auto.
+  rewrite (no_map_make_mono ((nodup_cancel _ _)++(nodup_cancel _ _))).
+  rewrite nodup_cancel_pointless. apply Permutation_trans with (l':=(nodup_cancel mono_eq_dec
+    (nodup_cancel mono_eq_dec (map make_mono (concat (map (substM s) q)))
+    ++ map make_mono (concat (map (substM s) (p)))))).
+    apply nodup_cancel_Permutation. apply Permutation_app_comm.
+  rewrite nodup_cancel_pointless. rewrite <- map_app. rewrite <- concat_app.
+  rewrite <- map_app. rewrite (no_map_make_mono (p++q)).
+  apply Permutation_trans with (l':=(nodup_cancel mono_eq_dec (map make_mono
+    (concat (map (substM s) (p++q)))))). apply nodup_cancel_Permutation.
+    apply Permutation_map. apply Permutation_concat. apply Permutation_map.
+    apply Permutation_app_comm.
+  apply Permutation_sym. repeat rewrite List.concat_map.
+  repeat rewrite map_map. apply nodup_cancel_concat_map.
+  intros x. rewrite no_map_make_mono. apply NoDup_MonoSorted; apply substM_is_poly.
+  intros m Hin; apply (substM_is_poly s x); auto.
+  intros m Hin; apply in_app_iff in Hin as []; destruct Hp; destruct Hq; auto.
+  intros m Hin; apply in_app_iff in Hin as []; apply nodup_cancel_in in H;
+  apply mono_in_map_make_mono in H; auto.
+Qed.
+
+Lemma substP_distr_mulPP : forall p q s,
+  substP s (mulPP p q) = mulPP (substP s p) (substP s q).
+Proof.
+  intros p q s. repeat rewrite mulPP_mulPP''. unfold substP, mulPP''.
+  apply Permutation_sort_eq. apply Permutation_trans with (l':=(nodup_cancel
+    mono_eq_dec (map make_mono (concat (map (substM s) (nodup_cancel mono_eq_dec
+    (map make_mono (concat (map (mulMP' p) q))))))))). apply nodup_cancel_Permutation.
+    apply Permutation_map. apply Permutation_concat. apply Permutation_map.
+    unfold make_poly. rewrite <- Permutation_MonoSort_l. auto.
+  apply Permutation_sym. apply Permutation_trans with (l':=(nodup_cancel
+    mono_eq_dec (map make_mono (concat (map (mulMP' (make_poly (concat (map
+    (substM s) p)))) (nodup_cancel mono_eq_dec (map make_mono (concat (map
+    (substM s) q))))))))). apply nodup_cancel_Permutation. apply Permutation_map.
+    apply Permutation_concat. apply Permutation_map. unfold make_poly.
+    rewrite <- Permutation_MonoSort_l. auto.
+  apply Permutation_sort_eq. rewrite make_poly_refold. rewrite mulPP''_refold.
+  rewrite <- mulPP_mulPP''. rewrite mulPP_comm. rewrite mulPP_mulPP''.
+  apply Permutation_sort_eq. apply Permutation_trans with (l':=(nodup_cancel
+    mono_eq_dec (map make_mono (concat (map (mulMP' (nodup_cancel mono_eq_dec
+    (map make_mono (concat (map (substM s) q))))) (nodup_cancel mono_eq_dec
+    (map make_mono (concat (map (substM s) p))))))))). apply nodup_cancel_Permutation.
+    apply Permutation_map. apply Permutation_concat. apply Permutation_map.
+    unfold make_poly. rewrite <- Permutation_MonoSort_l. auto.
+  apply Permutation_sym. 
+(*   intros p q s. repeat rewrite mulPP_mulPP''. induction q; auto.
+  unfold mulPP''. simpl. unfold substP. simpl. *)
+Admitted.
 
 Definition unifier (s : subst) (p : poly) : Prop :=
   substP s p = [].
@@ -271,16 +362,20 @@ Lemma appSubst_poly : forall x s,
   is_poly_subst s ->
   is_poly (appSubst s x).
 Proof.
-Admitted.
+  intros x s H. unfold is_poly_subst in H. induction s.
+  - simpl. auto.
+  - simpl. destruct a eqn:Ha. destruct (x =? v).
+    + apply (H v). intuition.
+    + apply IHs. intros x0 p0 H0. apply (H x0). intuition.
+Qed.
 
 Lemma subst_var : forall x s,
   is_poly_subst s ->
   substP s [[x]] = appSubst s x.
 Proof.
   intros. simpl.
-  apply (appSubst_poly x s) in H.
-  rewrite mulPP_1r; auto.
-  rewrite addPP_0r; auto.
+  apply (appSubst_poly x s) in H. unfold substP. simpl. rewrite app_nil_r.
+  rewrite mulPP_1r; auto. rewrite no_make_poly; auto.
 Qed.
 
 Lemma subst_comp_poly : forall s t u,
@@ -292,8 +387,9 @@ Lemma subst_comp_poly : forall s t u,
 Proof.
   intros. induction p.
   - simpl. auto.
-  - simpl. rewrite substP_distr_addPP; auto.
-    f_equal.
+  - simpl. unfold substP at 2. simpl. rewrite <- make_poly_pointless_r.
+    rewrite addPP_refold. rewrite substP_distr_addPP; auto. unfold substP at 3.
+    simpl. rewrite <- make_poly_pointless_r. rewrite addPP_refold. f_equal.
     + induction a.
       * simpl. auto.
       * simpl. rewrite substP_distr_mulPP.
@@ -301,7 +397,7 @@ Proof.
         -- rewrite <- subst_var; auto.
            rewrite <- subst_var; auto.
         -- apply IHa.
-    + apply IHp.
+    + rewrite substP_refold. apply IHp.
 Qed.
 
 Lemma reprod_is_mgu : forall p s,
@@ -312,7 +408,7 @@ Proof.
   intros p s [].
   split; auto.
   intros.
-  exists t.
+  exists t0.
   intros.
   apply H0; auto.
 Qed.
@@ -335,7 +431,8 @@ Proof.
   intros.
   induction p.
   - auto.
-  - simpl. apply poly_cons in H as H0. destruct H0.
+  - unfold substP. simpl. apply poly_cons in H as H0. destruct H0.
+    rewrite <- make_poly_pointless_r. rewrite substP_refold.
     rewrite IHp; auto.
     rewrite empty_substM; auto.
     apply addPP_poly_cons; auto.
@@ -356,7 +453,7 @@ Proof.
   split.
   - apply empty_unifier.
   - intros.
-    exists t.
+    exists t0.
     intros.
     rewrite empty_substP; auto.
 Qed.
@@ -369,4 +466,3 @@ Proof.
   - intros.
     rewrite empty_substP; auto.
 Qed.
-
